Dirty FrodoKEM_AES experiment

frodo/code/Hacl.Impl.Frodo.Gen.fst
@@ -114,7 +114,7 @@ val frodo_gen_matrix_cshake:
   -> Stack unit
     (requires fun h -> live h seed /\ live h res /\ disjoint seed res)
     (ensures  fun h0 _ h1 ->
-      live h1 res /\ modifies (loc_buffer res) h0 h1 /\
+      modifies (loc_buffer res) h0 h1 /\
       as_matrix h1 res == S.frodo_gen_matrix_cshake (v n) (v seed_len) (as_seq h0 seed))
 [@"c_inline"]
 let frodo_gen_matrix_cshake n seed_len seed res =
@@ -127,6 +127,98 @@ let frodo_gen_matrix_cshake n seed_len seed res =
   pop_frame ();
   let h1 = ST.get () in
   Spec.Matrix.extensionality (as_matrix h1 res) (S.frodo_gen_matrix_cshake (v n) (v seed_len) (as_seq h0 seed))
+
+assume
+val aes128_key_expansion_sbox: key:buffer uint8 -> expanded_key:buffer uint8 -> sbox:buffer uint8 -> ST unit
+  (requires fun h0 -> True)
+  (ensures  fun h0 _ h1 -> modifies loc_none h0 h1)
+
+assume
+val aes128_encrypt_one_block:
+  cipher:buffer uint8 -> plain:buffer uint8 -> w:buffer uint8 -> sbox:buffer uint8 -> ST unit
+  (requires fun h0 -> True)
+  (ensures  fun h0 _ h1 -> modifies (loc_buffer cipher) h0 h1)
+
+
+[@CAbstractStruct]
+noeq type aes128_key_s =
+  | AES128_VALE: w:buffer uint8 -> sbox:buffer uint8 -> aes128_key_s
+
+let aes128_key = B.pointer aes128_key_s
+
+val aes128_create:
+    key:buffer uint8
+  -> ST aes128_key
+    (requires fun h0 -> True)
+    (ensures  fun h0 _ h1 -> modifies loc_none h0 h1)
+let aes128_create k =
+  let w    = B.malloc HS.root (u8 0) 176ul in
+  let sbox = B.malloc HS.root (u8 0) 256ul in
+  aes128_key_expansion_sbox k w sbox;
+  B.malloc HS.root (AES128_VALE w sbox) 1ul
+
+val aes128_compute:
+    key:aes128_key
+  -> plain:buffer uint8
+  -> cipher:buffer uint8
+  -> ST unit
+    (requires fun h0 -> B.live h0 key)
+    (ensures  fun h0 _ h1 -> modifies (loc_buffer cipher) h0 h1)
+let aes128_compute key plain cipher =
+  let k = !*key in
+  let AES128_VALE w sbox = k in
+  aes128_encrypt_one_block cipher plain w sbox
+
+val aes128_free:
+    key:aes128_key
+  -> ST unit
+    (requires fun h0 -> live h0 key)
+    (ensures  fun h0 _ h1 -> True)
+let aes128_free key =
+  let k = !*key in
+  let AES128_VALE w sbox = k in
+  B.free w;
+  B.free sbox;
+  B.free key
+
+val frodo_gen_matrix_aes:
+    n:size_t{0 < v n /\ v n * v n <= max_size_t}
+  -> seed_len:size_t{v seed_len > 0}
+  -> seed:lbytes seed_len
+  -> a:matrix_t n n
+  -> Stack unit
+    (requires fun h -> live h seed /\ live h a /\ disjoint seed a)
+    (ensures  fun h0 _ h1 -> modifies (loc_buffer a) h0 h1)
+let frodo_gen_matrix_aes n seed_len seed a =
+  push_frame();
+  let key = aes128_create seed in
+  let b:lbytes (size 16) = create #uint8 (size 16) (u8 0) in
+  let c:lbytes (size 16) = create #uint8 (size 16) (u8 0) in
+  let h0 = ST.get() in
+  Lib.Loops.for (size 0) n
+    (fun h1 i -> modifies (loc_union (loc_buffer b) (loc_buffer a)) h0 h1)
+    (fun i ->
+      let h1 = ST.get() in
+      Lib.Loops.for (size 0) (n /. size 8)
+        (fun h2 j -> modifies (loc_union (loc_buffer b) (loc_buffer a)) h1 h2)
+        (fun j ->
+          let j = j *! size 8 in
+          uint_to_bytes_le (sub b (size 0) (size 2)) (to_u16 (size_to_uint32 i));
+          uint_to_bytes_le (sub b (size 2) (size 2)) (to_u16 (size_to_uint32 j));
+          aes128_compute key b c;
+          a.[i, j +! size 0] <- uint_from_bytes_le (sub c (size 0)  (size 2));
+          a.[i, j +! size 1] <- uint_from_bytes_le (sub c (size 2)  (size 2));
+          a.[i, j +! size 2] <- uint_from_bytes_le (sub c (size 4)  (size 2));
+          a.[i, j +! size 3] <- uint_from_bytes_le (sub c (size 6)  (size 2));
+          a.[i, j +! size 4] <- uint_from_bytes_le (sub c (size 8)  (size 2));
+          a.[i, j +! size 5] <- uint_from_bytes_le (sub c (size 10) (size 2));
+          a.[i, j +! size 6] <- uint_from_bytes_le (sub c (size 12) (size 2));
+          a.[i, j +! size 7] <- uint_from_bytes_le (sub c (size 14) (size 2))
+        )
+    );
+  aes128_free key;
+  pop_frame()
+
 
 val frodo_gen_matrix_cshake_4x:
     n:size_t{0 < v n /\ 2 * v n <= max_size_t /\ 256 + v n < maxint U16 /\ v n * v n <= max_size_t}
